progress up to verify

proofs/specs/MLDSA.ec
@@ -10,7 +10,7 @@ type Leakage = [
    | CheckZ of bool
    | CheckH of bool ].
 
-module MLDSA(XOFA : XOF_RejNTTPoly, XOFS : XOF_RejBPoly, RO : LeakyRO) = {
+module MLDSA(XOFA : XOF_RejNTTPoly, XOFS : XOF_RejBPoly, XOFSIB : XOF_SIB, RO : LeakyRO) = {
    proc keygen_derand(eps : Bytes32.t) : BytesSK.t * BytesPK.t= {
      var sk,rho,rhop,_K,_A,s1,s2,t,t1,t0,pk,tr,epsp;
      epsp <- Bytes34.of_list (Bytes32.to_list eps ++ [W8.of_int kvec;W8.of_int lvec]);
@@ -45,7 +45,7 @@ module MLDSA(XOFA : XOF_RejNTTPoly, XOFS : XOF_RejBPoly, RO : LeakyRO) = {
        y <@ ExpandMask.sample(rhopp,kappa);
        w <- invnttv (ntt_mulmxv _A (nttv y));
        w1 <- polykvec_HighBits w;
-       ctl <@ RO.get(mu,w1Encode w1);
+       ctl <@ RO(XOFSIB).get(mu,w1Encode w1);
        (ct,c) <- ctl.`1;
        leakage <- leakage ++ [ RO ctl.`2] ;
        ch <- ntt c;
@@ -70,7 +70,7 @@ module MLDSA(XOFA : XOF_RejNTTPoly, XOFS : XOF_RejBPoly, RO : LeakyRO) = {
   }
 
   proc verify(pk : BytesPK.t, sigma : BytesSig.t, m : W8.t list) : bool = {
-    var rho,t1,ctl,ct,c,z,h,rb,_A,tr,mu,wapprox,w1,ctp;
+    var rho,t1,c,l,ct,z,h,rb,_A,tr,mu,wapprox,w1,ctp;
     w1 <- witness;
     rb <- false;
     (rho,t1) <@ PkEncDec.pkDecode(pk);
@@ -79,13 +79,12 @@ module MLDSA(XOFA : XOF_RejNTTPoly, XOFS : XOF_RejBPoly, RO : LeakyRO) = {
       _A <@ ExpandA(XOFA).sample(rho);
       tr <- H_tr pk;
       mu <- H_mu tr m;
-      ctl <@ RO.get(mu,w1Encode w1);
-      (ct,c) <- ctl.`1;
+      (c,l) <@ SampleInBall(XOFSIB).sample(ct); (* we don't care about leakage in verify *)
       wapprox <- invnttv (ntt_mulmxv _A (nttv z) - (ntt_smul (ntt c) (nttv (smul t1 (incoeff (2^d))))));
       w1 <- UseHint (oget h) wapprox;
       ctp <- H_ct mu (w1Encode w1);
       rb <- infnorm z (gamma1 - Beta);
-      rb <- rb && ct = ctp && hammw (oget h) w_hint;
+      rb <- rb && ct = ctp;
     }
     return rb;
   }
