proofs/x86-64/avx2/ml_dsa_65/sample/challenge.ec
@@ -1,0 +1,23 @@
+require import AllCore List.
+
+from Jasmin require import JModel_x86.
+
+from JazzEC require import Ml_dsa_65_avx2 Mldsa_65_prelude.
+
+from Spec require import GFq Rq Serialization Conversion Parameters VecMat
+                         Symmetric Sampling MLDSA_W32_Rep MLDSA.
+
+import PolyLVec PolyKVec PolyMat.
+import CDR Round Zq PolyReduceZq BigZMod.
+
+require import Array48 Array256.
+
+(* Equiv between the spec SampleInBall (with concrete MLDSA_XOF_SIB) and the
+   Jasmin sample____challenge. The seed is the 48-byte commitment hash. *)
+lemma sample_challenge_correct :
+    equiv [ SampleInBall(MLDSA_XOF_SIB).sample ~ M.sample____challenge :
+       arg{1} = BytesCT.of_list (to_list arg{2}.`2)
+       ==>
+       lifts_wpoly res{2} = res{1}.`1
+    ].
+admitted. (* FIXME *)
