proofs/x86-64/avx2/ml_dsa_65/verify.ec
@@ -1,0 +1,215 @@
+require import AllCore List IntDiv RealExp.
+
+from Jasmin require import JModel_x86.
+
+from JazzEC require import Ml_dsa_65_avx2 Mldsa_65_prelude Matrix_A Hashing
+                           Signature Challenge.
+
+require import CircuitBindings Bindings XArray48.
+
+from Spec require import GFq Rq Serialization Conversion Parameters VecMat
+                         Symmetric Sampling MLDSA_W32_Rep MLDSA.
+
+import PolyLVec PolyKVec PolyMat.
+import CDR Round Zq PolyReduceZq BigZMod.
+
+require import Array2 Array32 Array48 Array64 Array256 Array768 Array1280 Array1536
+               Array1920 Array1952 Array3309 Array7680.
+               require import WArray48.
+
+require import BitEncoding.
+from CryptoSpecs require import JWordList.
+import BitChunking.
+
+lemma compare_commitment_hashes_ll : islossless M.__compare_commitment_hashes.
+proof.
+proc.
+wp;while (0 <=  offset <= 48 /\ offset %% 16 = 0) (48 -  offset); last by auto => />; smt().
+auto => /> ; smt().
+qed.
+
+lemma compare_commitment_hashes_correct (_lhs _rhs : W8.t Array48.t) :
+    phoare [ M.__compare_commitment_hashes :
+        arg.`1 = _lhs /\ arg.`2 = _rhs
+        ==>
+        res = (if _lhs = _rhs then W64.of_int 0 else -W64.one)
+    ] = 1%r.
+proof.
+have hh : hoare [ M.__compare_commitment_hashes :
+    arg.`1 = _lhs /\ arg.`2 = _rhs
+    ==>
+    res = (if _lhs = _rhs then W64.of_int 0 else -W64.one) ].
++ proc => /=.
+  proc change 2 : { lhs_bytes <- if (0 <=  offset * 8 <= 48*8-128)
+                                  then BSWAS_48u8_128.sliceget lhs (offset * 8)
+                                  else get128_direct (WArray48.init8 (fun i => lhs.[i])) (offset); }.
+  + auto => /> &2.
+    case (0 <= offset{2} * 8 <= 256); last  by auto.
+    by move => ?; rewrite -BSWAS_48u8_128_slicegetE /#.
+  proc change 3 : { rhs_bytes <- if (0 <=  offset * 8 <= 48*8-128)
+                                  then BSWAS_48u8_128.sliceget rhs ( offset * 8)
+                                  else get128_direct (WArray48.init8 (fun i => rhs.[i])) (offset); }.
+  + auto => /> &2.
+    case (0 <= offset{2} * 8 <= 256); last by auto.
+    by move => ?; rewrite -BSWAS_48u8_128_slicegetE /#.
+  proc change ^while.1 : { lhs_bytes <- if (0 <= offset * 8 <= 48*8-128)
+                                         then BSWAS_48u8_128.sliceget lhs (offset * 8)
+                                         else get128_direct (WArray48.init8 (fun i => lhs.[i])) (offset); }.
+  + auto => /> &2.
+    case (0 <= offset{2} * 8 <= 256); last by auto.
+    by move => ?; rewrite -BSWAS_48u8_128_slicegetE /#.
+  proc change ^while.2 : { rhs_bytes <- if (0 <= offset * 8 <= 48*8-128)
+                                         then BSWAS_48u8_128.sliceget rhs (offset * 8)
+                                         else get128_direct (WArray48.init8 (fun i => rhs.[i])) (offset); }.
+  + auto => /> &2.
+    case (0 <= offset{2} * 8 <= 256); last by auto.
+    by move => ?; rewrite -BSWAS_48u8_128_slicegetE /#.
+  cfold 1;unroll for ^while.
+  cfold 12.
+  wp 12.
+  conseq (: _ ==> _lhs = _rhs <=> result = W64.of_int 65535).
+  + move => &hr [<- <-] rr [Hl Hr].
+    case (rr <> W64.of_int 65535); last first.
+    + move => HH; rewrite Hr //=.
+      move => ?; rewrite ifF 1:/# /=; smt(@W64 pow2_64).
+  by circuit.
+conseq compare_commitment_hashes_ll hh;smt().
+qed.
+
+
+lemma ml_dsa_65_verify_correct _m :
+    equiv [ MLDSA(MLDSA_XOFA, MLDSA_XOFS, MLDSA_XOF_SIB, SIB_RO).verify ~ M.ml_dsa_65_verify :
+       Glob.mem{2} = _m /\
+       arg{1}.`1 = BytesPK.of_list (to_list arg{2}.`1)
+    /\ arg{1}.`2 = BytesSig.init (fun i => arg{2}.`5.[i])
+    /\ W64.to_uint arg{2}.`2.[1] <= 255
+    /\ 0 <= arg{2}.`4
+    /\ to_uint context{2}.[0] + to_uint context{2}.[1] < 18446744073709551616
+    /\ message_pointer{2} + message_size{2} < 18446744073709551616
+    /\ arg{1}.`3 = [W8.zero; truncateu8 arg{2}.`2.[1]]
+                   ++ memread _m (W64.to_uint arg{2}.`2.[0]) (W64.to_uint arg{2}.`2.[1])
+                   ++ memread _m arg{2}.`3 arg{2}.`4
+       ==>
+       Glob.mem{2} = _m /\
+       res{1} = (res{2} = W64.of_int 0)
+   ].
+proof.
+have Hlvec := mldsa65_lvec.
+have Hkvec := mldsa65_kvec.
+proc => /=; conseq |>.
+
+sp 0 2.
+rcondt {2} ^if; 1: by auto => /> /#.
+inline {2} M.__verify_internal.
+sp 0 6.
+seq 1 9 : #pre; 1: by auto.
+sp 1 0.
+seq 1 0 : (#pre /\
+    rho{1} = Bytes32.of_list (take 32 (BytesPK.to_list pk{1})) /\
+    t1{1}  = KArray.init (fun i =>
+        SimpleBitUnpack
+          (take ((n * (q_bits-d)) %/ 8)
+                (drop (((n * (q_bits-d)) %/ 8) * i + 32) (BytesPK.to_list pk{1})))
+          (2^(q_bits - d) - 1))).
++ ecall{1} (pkDecode_corr pk{1}).
+  by auto.
+seq 1 1 : (#pre /\
+    ct{1} = BytesCT.init (fun i => signature{2}.[i]) /\
+    lifts_wpolylvec (lvec_unflatten256 signer_response{2}) = z{1} /\
+    (h{1} = None => result{2} = -W64.one) /\
+    (h{1} <> None =>
+        result{2} = W64.zero /\
+        liftu_wpolykvec (kvec_unflatten256 hints{2}) = oget h{1} /\
+        wpolykvec_urng (kvec_unflatten256 hints{2}) 2)).
++ ecall (signature_decode signature{2}).
+  by auto.
+
+if; last first.
++ by auto => /> &2 ????  ->; rewrite to_uint_eq /=  minus_one oneE /=.
++ auto => /> &1 &2 ???? H H0;split => H1; 1: by smt().
+  case (h{1} = None) => H2; last by smt().
+  have := H H2; rewrite H1 /=.
+  by rewrite to_uint_eq /= minus_one oneE /=.
+
+(* expand A *)
+seq 1 1 : (#pre /\
+      liftu_wpolymat (mat_unflatten256 matrix_A{2}) = _A{1} /\
+      wpolymat_urng (mat_unflatten256 matrix_A{2}) 1).
+  + ecall{1} (ExpandA_correct rho{1}).
+    ecall{2} (matrix_A_correct (Array32.init (fun i => verification_key{2}.[i]))).
+    auto => |> &1 &2 ??????? rr -> ?;congr.
+    apply Bytes32.tP => k kb.
+    do 2!(rewrite Bytes32.get_of_list //).
+    rewrite get_to_list initiE 1:/# /=.
+    rewrite nth_take 1,2:/# BytesPK.get_to_list /=.
+    by rewrite BytesPK.get_of_list 1:/# get_to_list.
+
+(* anticipate hashing *)
+swap {2} [6..7] -5.
+
+(* verification key hash. *)
+sp 1 0.
+seq 0 1 : (#pre /\
+      verification_key_hash{2} =
+        Array64.of_list witness (Bytes64.to_list (H_tr pk{1}))).
+  + ecall{2} (hash_verification_key_correct verification_key{2}).
+    by auto.
+
+(* message representative *)    
+sp 1 0.
+seq 0 1 : (#pre /\
+      message_representative{2} =
+        Array64.of_list witness (Bytes64.to_list mu{1})).
+  + ecall{2} (derive_message_representative_ph
+                 verification_key_hash{2}
+                 (memread _m context_pointer{2} context_size{2})
+                 (memread _m message_pointer{2} message_size{2})).
+    wp; skip => /> &1 &2 *; do split.
+    + by rewrite !size_memread /=; smt(W64.to_uint_cmp).
+    + by rewrite !size_memread /=; smt(W64.to_uint_cmp).
+    + by rewrite !size_memread /=; smt(W64.to_uint_cmp).
+    + by rewrite !size_memread /=;  smt(W64.to_uint_cmp).
+    move => ????;do congr.
+    + rewrite Bytes64.tP => k kb.
+      by rewrite Bytes64.get_of_list // get_to_list get_of_list //.
+    + by rewrite size_memread; smt(W64.to_uint_cmp).
+   
+(* anticipate sib *)
+swap {2} [3..4] -2.
+  seq 1 1 : (#pre /\ lifts_wpoly challenge{2} = c{1}).
+  + call sample_challenge_correct.
+    wp; skip => /> &1 &2 *.
+    rewrite BytesCT.tP => i ib.
+    rewrite BytesCT.initiE 1:/# BytesCT.get_of_list 1:/#.
+    by rewrite get_to_list initiE; smt(mldsa65_lambda).
+
+(* jump over algebra *)
+seq 2 4 :
+  (#pre /\
+    BytesW1.of_list (to_list reconstructed_signer_commitment{2}) = w1Encode w1{1}); last first.
+
+(* recompute hash *)
+sp 1 0.
+seq 0 1 : (#pre /\
+      expected_commitment_hash{2} =
+        Array48.of_list witness (BytesCT.to_list (H_ct mu{1} (w1Encode w1{1})))).
+  + ecall{2} (derive_commitment_hash_ph message_representative{2}
+                 reconstructed_signer_commitment{2}).
+    wp; skip => /> &1 &2 *; do congr.
+    rewrite Bytes64.tP => k kb.
+    + by rewrite Bytes64.get_of_list // get_to_list get_of_list //.
+
+ wp; ecall{2} (compare_commitment_hashes_correct expected_commitment_hash{2} (Array48.init (fun (i : int) => signature_encoded{2}.[0 + i]))).
+ 
+ wp;skip => /> &1 &2 *.
+ pose xx := H_ct
+   (H_mu (H_tr (BytesPK.of_list (to_list verification_key{2})))
+      (W8.zero :: truncateu8 context{2}.[1] :: (memread _m (to_uint context{2}.[0]) (to_uint context{2}.[1]) ++
+                                                memread _m message_pointer{2} message_size{2}))) (
+   w1Encode w1{1}). admit. (* Something's wrong *)
+ 
+
+(* algebra *)
+admit.
+
+qed.
