proofs/xarrays/XArray48.ec
@@ -1,0 +1,62 @@
+(* -------------------------------------------------------------------- *)
+require import AllCore List IntDiv JWordExtra JArrayExtra CircuitBindings.
+require (*--*) Array48.
+
+from Jasmin require import JWord.
+
+(* -------------------------------------------------------------------- *)
+clone export PAE with
+      op size <- 48,
+  theory A    <- Array48.Array48.
+
+(* -------------------------------------------------------------------- *)
+clone BSA as BSA48 with
+      op size <- 48,
+  theory A    <- Array48.Array48
+
+  proof gt0_size by done.
+
+(* -------------------------------------------------------------------- *)
+clone BSWA as BSWA_48u8 with
+      op asize <- 48,
+      op bsize <- 8,
+  theory A     <- Array48.Array48,
+  theory BSA   <- BSA48,
+  theory W     <- W8 { rename "_XX" as "_8" },
+  theory WE    <- WE8,
+  theory BSW   <- BSW8
+  proof *.
+
+(* -------------------------------------------------------------------- *)
+clone BSWAS as BSWAS_48u8_128 with
+      op asize   <- 48,
+      op bsize   <- 8,
+      op ssize   <- 128,
+  theory A       <- Array48.Array48,
+  theory BSA     <- BSA48,
+  theory WB      <- W8  { rename "_XX" as "_8" },
+  theory WEB     <- WE8,
+  theory BSWB    <- BSW8,
+  theory WS      <- W128  { rename "_XX" as "_128" },
+  theory WES     <- WE128,
+  theory BSWS    <- BSW128,
+  theory BSWA    <- BSWA_48u8
+
+  proof le_size by done.
+
+require import WArray48 BitEncoding.
+import Array48 BitChunking.
+
+lemma BSWAS_48u8_128_slicegetE o (p : W8.t Array48.t):
+    0 <= o*8 <= 48*8-128 =>
+     get128_direct (WArray48.init8 (fun (i_0 : int) => p.[i_0])) o = BSWAS_48u8_128.sliceget p (o * 8).
+proof.
+move => Ho.
+rewrite /get128_direct /pack16_t;apply W128.wordP => k kb.
+have //= := BSWAS_48u8_128.BVA_asliceget_Top_CircuitBindings_BSWAS_WB_t_Top_CircuitBindings_BSWAS_WS_t_Top_CircuitBindings_BSWAS_A_t.bvaslicegetP p (o * 8) _; 1: by smt().
+move => -> //; rewrite initiE 1:/# /= initiE 1:/# /= initiE 1:/# /=.
+rewrite nth_take 1,2:/# nth_drop 1,2:/#  (nth_flatten false 8).
++ rewrite allP /= => x; rewrite mapP => He; elim He;smt(W8.size_w2bits).
+rewrite (nth_map witness); 1: by rewrite size_to_list; smt().
+by rewrite get_to_list get_w2bits /#.
+qed.
